lambda2Gmu/Progress.v
@@ -87,6 +87,7 @@ Theorem progress_thm : progress.
   - right.
     eexists.
     constructor*.
+  - admit.
   - IHT e1.
     right. destruct IHt as [Hv | Hev].
     + eexists. econstructor; eauto.
@@ -94,4 +95,4 @@ Theorem progress_thm : progress.
       eexists; eapply ered_let; eauto.
 
   - eapply typing_implies_term; eauto.
-Qed.
+Admitted.
